wip, with jared

ulib/FStar.ST.fst
@@ -21,6 +21,7 @@ open FStar.Preorder
 open FStar.DataInvariant
 
 (***** Global ST (GST) effect with put, get, witness, and recall *****)
+type iheap = h:heap{forall r. h `contains` r ==> invariant_of h1 r (sel h1 r)}
 
 new_effect GST = STATE_h heap
 
@@ -31,10 +32,24 @@ let gst_wp (a:Type)   = st_wp_h heap a
 unfold let lift_div_gst (a:Type0) (wp:pure_wp a) (p:gst_post a) (h:heap) = wp (fun a -> p a h)
 sub_effect DIV ~> GST = lift_div_gst
 
-let heap_rel (h1:heap) (h2:heap) =
-  forall (a:Type0) (inv:data_inv a) (rel:preorder a) (r:mref a inv rel). h1 `contains` r ==>
-                                               (h2 `contains` r /\ rel (sel h1 r) (sel h2 r))
+let related_at (h1:heap) (h2:heap) (a:Type0) (inv:data_inv a) (rel:preorder a) (r:mref a inv rel) = 
+           h1 `contains` r ==>
+           (h2 `contains` r /\ rel (sel h1 r) (sel h2 r))
 
+let heap_rel (h1:heap) (h2:heap) =
+  forall (a:Type0) (inv:data_inv a) (rel:preorder a) (r:mref a inv rel).
+    related_at h1 h2 a inv rel r
+
+let forall_intro_4 (#a:Type) (#b:(a -> Type)) (#c:(x:a -> y:b x -> Type)) (#d:(x:a -> y:b x -> z:c x y -> Type)) (#p:(x:a -> y:b x -> z:c x y -> w:d x y z -> Type0))
+		  ($f: (x:a -> y:b x -> z:c x y -> w:d x y z -> Lemma (p x y z w)))
+  : Lemma (forall (x:a) (y:b x) (z:c x y) (w:d x y z). p x y z w)
+  = let g : x:a -> Lemma (forall (y:b x) (z:c x y) (w:d x y z). p x y z w) = fun x -> FStar.Classical.forall_intro_3 (f x) in
+    FStar.Classical.forall_intro g
+
+let intro_heap_rel (h1:heap) (h2:heap) (f: (a:Type0) -> (inv:data_inv a) -> (rel:preorder a) -> (r:mref a inv rel) -> Lemma (related_at h1 h2 a inv rel r))
+  : Lemma (heap_rel h1 h2)
+  = forall_intro_4 f
+  
 assume val gst_get: unit    -> GST heap (fun p h0 -> p h0 h0)
 assume val gst_put: h1:heap -> GST unit (fun p h0 -> heap_rel h0 h1 /\ p () h1)
 
@@ -92,26 +107,67 @@ abstract let read (#a:Type) (#inv:data_inv a) (#rel:preorder a) (r:mref a inv re
     gst_recall (contains_pred r);
     sel_tot h0 r
 
-let upd_maintains_heap_inv (b:Type0) (inv_b:data_inv b) (rel_b:preorder b) (r':mref b inv_b rel_b) (v:b) (h1 h2 : heap):
+let upd_maintains_heap_inv (b:Type0) (inv_b:data_inv b) (rel_b:preorder b) (r':Heap.mref b inv_b rel_b) (v:b) (h1 h2 : heap):
 (a:Type0) ->
 (inv:data_inv a) ->
 (rel:preorder a) ->
-(r:mref a inv rel) ->
-Lemma (requires h2 == upd h1 r' v) (ensures (h1 `contains` r ==> (h2 `contains` r /\ rel (sel h1 r) (sel h2 r)))) =
-fun a inv rel r ->
+(r:Heap.mref a inv rel) ->
+Lemma (requires h2 == upd h1 r' v) 
+      (ensures (related_at h1 h2 a inv rel r)) //(h1 `contains` r ==> (h2 `contains` r /\ rel (sel h1 r) (sel h2 r)))) =
+= fun a inv rel r ->
 if compare_addrs r r'
 then (assume (h2 `contains` r); assume (rel (sel h1 r) (sel h2 r)))
 else ()
 
 
-#set-options "--ugly --print_effect_args --print_full_names"
+(* #reset-options // "--ugly --print_effect_args --print_full_names" *)
 
-let upd_tot_maintains_heap_inv (#b:Type) (#inv_b:data_inv b) (#rel_b:preorder b) (r':mref b inv_b rel_b) (v:b) (h0 h1 : heap) :
+
+
+(* #set-options "--z3rlimit 30" *)
+
+let upd_tot_maintains_heap_inv (#b:Type) (#inv_b:data_inv b) (#rel_b:preorder b) (r':Heap.mref b inv_b rel_b) (v:b) (h0 h1 : heap) :
 Lemma
   (requires (h1 == upd h0 r' v))
   (ensures (heap_rel h0 h1)) =
+  let aux (a : Type0) (inv:data_inv a) (rel:preorder a) (r:Heap.mref a inv rel) : 
+    Lemma (related_at h0 h1 a inv rel r) =
+    upd_maintains_heap_inv b inv_b rel_b r' v h0 h1 a inv rel r
+  in
+  forall_intro_4 aux
+  
+  
+  assert (forall (a : Type0) (inv:data_inv a) (rel:preorder a) (r:mref a inv rel). related_at h0 h1 a inv rel r);
+  intro_heap_rel h0 h1;  admit()
+  
+  assert (heap_rel h0 h1);
+  admit()
+  
+  
+  assert (forall (a : Type0) (inv:data_inv a) (rel:preorder a) (r:mref a inv rel). h0 `contains` r ==> (h1 `contains` r /\ rel (sel h0 r) (sel h1 r)))
+  
+  intro_heap_rel h0 h1
+  
+
+  assert (heap_rel h0 h1);
+  admit()
+
+  
+  (fun (a : Type0) (inv:data_inv a) (rel:preorder a) (r:mref a inv rel) -> 
+    
+  let _ = fun 
+    (FStar.Classical.forall_intro 
+      (FStar.Classical.move_requires (fun (r:mref a inv rel) -> upd_maintains_heap_inv b inv_b rel_b r' v h0 h1 a inv rel))) in
+   admit()
+   
+      
+      
+      r)) in 
+  admit()
+    
+    
 FStar.Classical.forall_intro_3 (fun (a : Type0) (inv:data_inv a) (rel:preorder a) ->
-  (FStar.Classical.forall_intro (fun (r:mref a inv rel) -> upd_maintains_heap_inv b inv_b rel_b r' v h0 h1 a inv rel r))) <: Lemma (requires (h1 == upd h0 r' v))
+  ) <: Lemma (requires (h1 == upd h0 r' v))
                                                                                                                (ensures (heap_rel h0 h1))
 
 abstract let write (#a:Type) (#inv:data_inv a) (#rel:preorder a) (r:mref a inv rel) (v:a)
